cedar-lean/Cedar/Slice/PolicySlice.lean
@@ -14,7 +14,9 @@
  limitations under the License.
 -/
 
-import Cedar.Spec
+module
+
+public import Cedar.Spec
 
 /-!
 This file defines a simple policy slicing algorithm that is based
@@ -28,11 +30,11 @@ open Cedar.Spec
 /--
 A policy bound consists of optional `principal` and `resource` entities.
 -/
-structure PolicyBound where
+public structure PolicyBound where
   principalBound : Option EntityUID
   resourceBound  : Option EntityUID
 
-def inSomeOrNone (uid : EntityUID) (opt : Option EntityUID) (entities : Entities) : Bool :=
+public def inSomeOrNone (uid : EntityUID) (opt : Option EntityUID) (entities : Entities) : Bool :=
   match opt with
   | .some uid' => inₑ uid uid' entities
   | .none      => true
@@ -42,7 +44,7 @@ A bound is satisfied by a request and store if the request principal and
 resource fields are descendents of the corresponding bound fields (or if those
 bound fields are `none`).
 -/
-def satisfiedBound (bound : PolicyBound) (request : Request) (entities : Entities) : Bool :=
+public def satisfiedBound (bound : PolicyBound) (request : Request) (entities : Entities) : Bool :=
   inSomeOrNone request.principal bound.principalBound entities ∧
   inSomeOrNone request.resource bound.resourceBound entities
 
@@ -50,21 +52,21 @@ def satisfiedBound (bound : PolicyBound) (request : Request) (entities : Entitie
 /--
 A bound analysis takes as input a policy and returns a PolicyBound.
 -/
-abbrev BoundAnalysis := Policy → PolicyBound
+public abbrev BoundAnalysis := Policy → PolicyBound
 
 /--
 A bound-based slicing algorithm takes as input a bound analysis, request, entities,
 and policies, and filters out the policies whose bound is not satisfied by the
 request and entities.
 -/
-def BoundAnalysis.slice (ba : BoundAnalysis) (request : Request) (entities : Entities) (policies : Policies) : Policies :=
+public def BoundAnalysis.slice (ba : BoundAnalysis) (request : Request) (entities : Entities) (policies : Policies) : Policies :=
   policies.filter (fun policy => satisfiedBound (ba policy) request entities)
 
 
 /--
 Scope-based bound analysis extracts the bound from the policy scope.
 -/
-def scopeAnalysis (policy : Policy) : PolicyBound :=
+public def scopeAnalysis (policy : Policy) : PolicyBound :=
   {
     principalBound := policy.principalScope.scope.bound,
     resourceBound  := policy.resourceScope.scope.bound,
